sepcomp/pred_lemmas.v
@@ -1,41 +1,241 @@
+Require Import Bool.
+
 Require Import ssreflect ssrbool ssrnat ssrfun eqtype seq fintype finfun.
 Set Implicit Arguments.
 Unset Strict Implicit.
 Unset Printing Implicit Defensive.
 
-(* I'm probably missing these in the ssreflect libraries ... *)
+Require Import msl.Axioms.
 
+(* A small library of lemmas on Ssreflect boolean predicates, all assuming 
+   function extensionality so we can state the lemmas in rewrite form. *)
+
+Notation Disjoint p q := ([predI p & q] = pred0).
+
+Notation Disjoint_ext p q := ([predI p & q] =i pred0).
+ 
 Section pred_lems.
 
-Context {T} {pTy : predType T} (p q r : pTy).
+Variable T : Type.
 
-Lemma predI0 : [predI p & pred0] =i pred0.
-Proof. by rewrite/eq_mem/=/in_mem/=/andb=> x; case: (x \in p). Qed.
-
-Lemma predIT : [predI predT & p] =i p.
-Proof. by rewrite/eq_mem/=/in_mem/=/andb/in_mem => x. Qed.
-
-Lemma predIC : [predI p & q] =i [predI q & p].
+Lemma pred_ext (p q : pred T) : p = q <-> p =i q.
 Proof. 
-by rewrite/eq_mem/in_mem/=/andb=> x; case: (x \in p); case: (x \in q).
+split=> A; first by move=> b; rewrite A.
+by extensionality b; apply: (A b).
 Qed.
 
-Lemma in_predI b : b \in [predI p & q] = [&& b \in p & b \in q].
+Lemma pred_eta (p : pred T) : p = [pred x | p x].
+Proof. by extensionality a. Qed.
+
+Lemma pred_exteta (p q : pred T) :
+  [pred x | p x] = [pred x | q x] <-> [pred x | p x] =i [pred x | q x].
+Proof. 
+split=> A; first by move=> b; rewrite A.
+by f_equal; extensionality b; apply: (A b).
+Qed.
+
+Lemma predIC (p q : pred T) : [predI p & q] = [predI q & p].
+Proof. by rewrite/predI; f_equal; extensionality a; rewrite andb_comm. Qed.
+
+Lemma predIA (p q r : pred T) : 
+  [predI p & [predI q & r]] = [predI [predI p & q] & r].
+Proof.
+rewrite/predI/in_mem/=; f_equal; extensionality a.
+by rewrite/in_mem/=; case: (p a); case: (q a); case: (r a).
+Qed.
+
+Lemma predI02 (p : pred T) : [predI pred0 & p] = pred0.
+Proof. by rewrite/predI/pred0; f_equal; extensionality a=> /=. Qed.
+
+Lemma predI01 (p : pred T) : [predI p & pred0] = pred0.
+Proof. by rewrite predIC predI02. Qed.
+
+Lemma predIT2 (p : pred T) : [predI predT & p] = [pred x | p x].
+Proof. by []. Qed.
+
+Lemma predIT1 (p : pred T) : [predI p & predT] = [pred x | p x].
+Proof. by rewrite predIC predIT2. Qed.
+
+Lemma predI_sub1 (p q r : pred T) : 
+  {subset p <= [predI q & r]} -> 
+  {subset p <= q} /\ {subset p <= r}.
+Proof.
+by move=> A; split=> a B; move: (A a B); rewrite/in_mem/=; move/andP=> [].
+Qed.
+
+Lemma predI_sub2 (p q : pred T) : 
+  [predI p & q] = [pred x | p x] -> {subset p <= q}.
+Proof.
+rewrite pred_exteta=> A a; move: (A a); rewrite/in_mem/=; move/andP.
+by rewrite/in_mem/=; case: (p a)=> // [][].
+Qed.
+
+Lemma predI_sub3 (p p' q : pred T) : 
+  [predI p & q] = [pred x | p x] -> 
+  {subset p' <= p} -> 
+  [predI p' & q] = [pred x | p' x].
+Proof.
+rewrite !pred_exteta=> A B a; move: (A a) (B a); rewrite/in_mem/=.
+move/andP; rewrite/in_mem/=. 
+case: (p a); case: (p' a); case: (q a)=> //; first by case.
+by move=> _; move/(_ erefl).
+Qed.
+
+Lemma in_predI (p q : pred T) b : 
+  b \in [predI p & q] = [&& b \in p & b \in q].
 Proof. by rewrite/in_mem. Qed.
+
+Lemma predUC (p q : pred T) : [predU p & q] = [predU q & p].
+Proof. by rewrite/predU; f_equal; extensionality a; rewrite orb_comm. Qed.
+
+Lemma predUA (p q r : pred T) : 
+  [predU p & [predU q & r]] = [predU [predU p & q] & r].
+Proof.
+rewrite/predU/in_mem/=; f_equal; extensionality a.
+by rewrite/in_mem/=; case: (p a); case: (q a); case: (r a).
+Qed.
+
+Lemma predU02 (p : pred T) : [predU pred0 & p] = [pred x | p x].
+Proof. by rewrite/predU/pred0; f_equal; extensionality a=> /=. Qed.
+
+Lemma predU01 (p : pred T) : [predU p & pred0] = [pred x | p x].
+Proof. by rewrite predUC predU02. Qed.
+
+Lemma predUT2 (p : pred T) : [predU predT & p] = predT.
+Proof. by []. Qed.
+
+Lemma predUT1 (p : pred T) : [predU p & predT] = predT.
+Proof. by rewrite predUC predUT2. Qed.
+
+Lemma in_predU (p q : pred T) b : 
+  b \in [predU p & q] = [|| b \in p | b \in q].
+Proof. by rewrite/in_mem. Qed.
+
+Lemma predD02 (p : pred T) : [predD pred0 & p] = pred0.
+Proof. 
+rewrite/predD/pred0; f_equal; extensionality a=>/=.
+by rewrite/in_mem/=; rewrite andb_false_r.
+Qed.
+
+Lemma predD01 (p : pred T) : [predD p & pred0] = [pred x | p x].
+Proof. by []. Qed.
+
+Lemma predDT2 (p : pred T) : [predD predT & p] = [pred x | ~~p x].
+Proof. 
+rewrite/predD/predT; f_equal; extensionality a=>/=.
+by rewrite/in_mem/=; rewrite andb_true_r.
+Qed.
+
+Lemma predDT1 (p : pred T) : [predD p & predT] = pred0.
+Proof. by []. Qed.
+
+Lemma predDI1 (p q : pred T) : [predI [predD p & q] & q] = pred0.
+Proof.
+rewrite/predI/predD/pred0/=; f_equal; extensionality a.
+by rewrite/in_mem/= andb_comm andb_assoc andb_negb_r.
+Qed.
+
+Lemma predDI2 (p q : pred T) : [predI q & [predD p & q]] = pred0.
+Proof. by rewrite predIC predDI1. Qed.
+
+Lemma predDU1 (p q : pred T) : [predU [predD p & q] & q] = [predU p & q].
+Proof.
+rewrite/predU/predD/=; f_equal; extensionality a.
+by rewrite/in_mem/=; case: (p a); case: (q a).
+Qed.
+
+Lemma predDU2 (p q : pred T) : [predU q & [predD p & q]] = [predU p & q].
+Proof. by rewrite (predUC q) predDU1. Qed.
+
+Lemma predDidem (p q : pred T) : 
+  [predD [predD p & q] & q] = [predD p & q].
+Proof.
+rewrite/predD; f_equal; extensionality a=>/=.
+by rewrite/in_mem/= -{3}(andb_diag (~~ q a)) andb_assoc.
+Qed.
+
+Lemma in_predD (p q : pred T) b : 
+  b \in [predD p & q] = [&& b \in p & b \notin q].
+Proof. by rewrite/in_mem/=/in_mem/= andb_comm. Qed.
+
+Lemma DisjointIn1 (p q : pred T) : 
+  [predD p & q]=[pred x | p x] -> Disjoint p q.
+Proof.
+move=> A; change ([predI [pred x | p x] & q] = pred0).
+by rewrite -A predDI1.
+Qed.
+
+Lemma DisjointInD (p q : pred T) : Disjoint [predD p & q] q.
+Proof. by apply: DisjointIn1; rewrite predDidem. Qed.
+
+Lemma DisjointInE (p q : pred T) : 
+  Disjoint p q <-> Disjoint_ext p q.
+Proof. 
+rewrite/predI/pred0/=; split=> A; f_equal; first by rewrite A.
+by extensionality a; apply: (A a).
+Qed.
+
+Lemma DisjointInI (p q : pred T) : Disjoint [predI p & q] [pred a | ~~ q a].
+Proof. 
+rewrite DisjointInE=> a; rewrite/predI/pred0/=/in_mem/=.
+by case: (p a); case: (q a)=> //.
+Qed.
+
+Lemma DisjointC (p q : pred T) : Disjoint p q <-> Disjoint q p.
+Proof. by split=> A; rewrite predIC. Qed.
+
+Lemma DisjointP (p q : pred T) : Disjoint p q <-> forall a, ~ p a \/ ~ q a.
+Proof.
+rewrite DisjointInE; split;
+move=> A a; move: (A a); rewrite in_predI /in_mem/=.
+by rewrite andb_false_iff; case=> ->; [left|right].
+rewrite andb_false_iff; case=> B; [left|right].
+by move: B; case: (p a).
+by move: B; case: (q a).
+Qed.
+
+Lemma Disjoint_incr (p q r : pred T) : 
+  Disjoint p q -> 
+  Disjoint p [predD r & q] -> 
+  Disjoint p r.
+Proof.
+move/DisjointP=> A; move/DisjointP=> B; rewrite DisjointP=> a.
+move: (A a) (B a); case; first by left.
+move=> C; case=> D; first by left.
+move: C D; rewrite/predD/=/in_mem/=. 
+by case: (q a)=> //; case: (r a)=> //; right.
+Qed.
+
+Lemma Disjoint_sub1 (p q q' : pred T) :
+  Disjoint p q -> 
+  {subset q' <= q} -> 
+  Disjoint p q'.
+Proof.
+move/DisjointP=> A B; rewrite DisjointP=> a; move: (A a) (B a).
+rewrite/in_mem/=; case: (p a); case: (q a); case: (q' a);
+try solve[by left|by right|by case].
+by move=> _; elim=> //; left.
+Qed.
+
+Lemma Disjoint_sub2 (p p' q : pred T) :
+  Disjoint p q -> 
+  {subset p' <= p} -> 
+  Disjoint p' q.
+Proof.
+move/DisjointP=> A B; rewrite DisjointP=> a; move: (A a) (B a).
+rewrite/in_mem/=; case: (p a); case: (q a); case: (p' a);
+try solve[by left|by right|by case].
+by move=> _; elim=> //; left.
+Qed.
 
 Lemma in_pred0 (b : T) : b \in pred0 = false.
 Proof. by rewrite/pred0/in_mem. Qed.
 
-Lemma eq_mem_trans : p =i q -> q =i r -> p =i r.
-Proof. 
-by rewrite/eq_mem/in_mem/= => H H2 x; rewrite -(H2 x) (H x). 
-Qed.
-
-Lemma my_subset_trans : 
+Lemma subset_trans' (p q r : pred T) : 
   {subset p <= q} -> {subset q <= r} -> {subset p <= r}.
 Proof. by move=> A B b C; apply: B; apply: A. Qed.
 
-Lemma subsetI :
+Lemma subsetI (p q r : pred T) :
   {subset p <= q} -> {subset p <= r} -> {subset p <= [predI q & r]}.
 Proof.
 move=> A B b C; apply/andP=> /=; split; first by apply: A.
